perf: improve bv_decide performance with large literals

src/Std/Tactic/BVDecide/Bitblast/BVExpr/Basic.lean
@@ -293,8 +293,15 @@ The semantics for `BVExpr`.
 -/
 def eval (assign : Assignment) : BVExpr w → BitVec w
   | .var idx =>
-    let ⟨bv⟩ := assign.get idx
-    bv.truncate w
+    let packedBv := assign.get idx
+    /-
+    This formulation improves performance, as in a well formed expression the condition always holds
+    so there is no need for the more involved `BitVec.truncate` logic.
+    -/
+    if h : packedBv.w = w then
+      h ▸ packedBv.bv
+    else
+      packedBv.bv.truncate w
   | .const val => val
   | .zeroExtend v expr => BitVec.zeroExtend v (eval assign expr)
   | .extract start len expr => BitVec.extractLsb' start len (eval assign expr)
@@ -308,8 +315,13 @@ def eval (assign : Assignment) : BVExpr w → BitVec w
   | .arithShiftRight lhs rhs => BitVec.sshiftRight' (eval assign lhs) (eval assign rhs)
 
 @[simp]
-theorem eval_var : eval assign ((.var idx) : BVExpr w) = (assign.get idx).bv.truncate _ := by
-  rfl
+theorem eval_var : eval assign ((.var idx) : BVExpr w) = (assign.get idx).bv.truncate w := by
+  rw [eval]
+  split
+  · next h =>
+    subst h
+    simp
+  · rfl
 
 @[simp]
 theorem eval_const : eval assign (.const val) = val := by rfl
